theories/aneris_lang/lib/nodup.v
@@ -1,0 +1,82 @@
+From aneris.aneris_lang Require Import proofmode notation.
+From aneris.aneris_lang.lib Require Import util set network_util.
+From iris_string_ident Require Import ltac2_string_ident.
+Set Default Proof Using "Type".
+Import Network.
+
+Definition receivefrom_nodup : val :=
+  λ: "socket" "msgs",
+  (rec: "loop" <> :=
+     let: "msg" := unSOME (ReceiveFrom "socket") in
+     if: set_mem "msg" "msgs" then "loop" #()
+     else ("msg", set_add "msg" "msgs")) #().
+
+Definition nodup_init : val := set_empty.
+
+Section nodup_specs.
+  Context `{dG : anerisG Mdl Σ}.
+
+  Local Definition msg_toval : message_body * socket_address → val :=
+    λ '(b, s), (#b, #s)%V.
+
+  Local Instance: Inj (=) (=) msg_toval.
+  Proof. intros [] []. by inversion 1; simplify_eq. Qed.
+
+  Definition is_nodup (R : gset message) (a : socket_address) (v : val) : Prop :=
+    is_set msg_toval (gset_map (λ m, (m_body m, m_sender m)) R) v ∧
+    set_Forall (λ m, m_destination m = a) R.
+
+  Lemma wp_nodup_init a :
+    {{{ True }}}
+      nodup_init #() @[ip_of_address a]
+    {{{ v, RET v; ⌜is_nodup (∅ : gset message) a v⌝ }}}.
+  Proof.
+    iIntros (Φ) "_ HΦ".
+    wp_apply (wp_set_empty msg_toval); [done|].
+    iIntros (??).
+    iApply "HΦ". eauto.
+  Qed.
+
+  Lemma wp_receivefrom_nodup ip a φ h s R T v :
+    ip = ip_of_address a →
+    saddress s = Some a →
+    sblock s = true →
+    {{{ h ↪[ip] s ∗ a ⤇ φ ∗ a ⤳ (R, T) ∗ ⌜is_nodup R a v⌝ }}}
+      receivefrom_nodup #(LitSocket h) v @[ip]
+    {{{ m v', RET ((#(m_body m), #(m_sender m)), v')%V;
+          h ↪[ip] s ∗ a ⤳ ({[m]} ∪ R, T) ∗ ⌜is_nodup ({[m]} ∪ R) a v'⌝ ∗ φ m }}}.
+  Proof.
+    iIntros (-> ?? Φ) "(Hh & #Hφ & Ha & [%Hv %Hdest]) HΦ".
+    wp_rec. do 3 wp_pure _.
+    iLöb as "IH" forall (R Hv Hdest).
+    wp_pures.
+    wp_apply (aneris_wp_receivefrom with "[$Hh $Hφ $Ha]"); [done..|].
+    iIntros (?) "[%Hd [(%Hm & Hh & Ha & _ & Hm) | (%Hm & Hh & Ha)]]".
+    - wp_apply wp_unSOME; [done|]; iIntros "_".
+      wp_pures.
+      wp_apply (wp_set_mem msg_toval _ (_,_) with "[//]").
+      iIntros ([] Hb).
+      { apply gset_map_correct2 in Hb.
+        destruct Hb as [m' [? Hm']].
+        rewrite -(Hdest _ Hm') in Hd.
+        simplify_eq.
+        by rewrite (message_inv m m') in Hm. }
+      wp_pures.
+      wp_apply (wp_set_add msg_toval _ (_,_) with "[//]").
+      iIntros (v' Hv').
+      wp_pures. iApply "HΦ".
+      iFrame. iPureIntro.
+      rewrite -(gset_map_singleton (λ m, (m_body m, m_sender m)) m) -gset_map_union in Hv'.
+      split; auto.
+      intros ? [-> %elem_of_singleton_1 | ?]%elem_of_union; [done|].
+      by apply Hdest.
+    - wp_apply wp_unSOME; [done|]; iIntros "_".
+      wp_pures.
+      wp_apply (wp_set_mem msg_toval _ (_,_) with "[//]").
+      iIntros ([] Hb); last first.
+      { by apply (gset_map_correct1 (λ m, (m_body m, m_sender m))) in Hm. }
+      wp_if.
+      iApply ("IH" with "[//] [//] Hh Ha HΦ").
+  Qed.
+
+End nodup_specs.
