theories/aneris_lang/lib/set.v
@@ -1,0 +1,51 @@
+From aneris.aneris_lang Require Import proofmode.
+From aneris.aneris_lang.lib Require Import list.
+Set Default Proof Using "Type".
+
+Definition set_empty : val := λ: <>, [].
+Definition set_add : val := list_cons.
+Definition set_mem : val := list_mem.
+
+Section set_specs.
+  Context `{anerisG Mdl Σ}.
+  Context `{Countable A}.
+  Context (toval : A → val).
+
+  Definition is_set (X : gset A) (v : val) : Prop :=
+    ∃ (l : list A), is_list (map toval l) v ∧ X = list_to_set l.
+
+  Lemma wp_set_empty  ip :
+    {{{ True }}}
+      set_empty #() @[ip]
+    {{{ v, RET v; ⌜is_set ∅ v⌝}}}.
+  Proof.
+    iIntros (Φ) "_ HΦ".
+    wp_rec. wp_pures. iApply "HΦ".
+    iExists []. repeat iSplit; auto.
+  Qed.
+
+  Lemma wp_set_add ip x X v :
+    {{{ ⌜is_set X v⌝ }}}
+      set_add (Val (toval x)) (Val v) @[ip]
+    {{{ v, RET v; ⌜is_set ({[ x ]} ∪ X) v⌝}}}.
+  Proof.
+    iIntros (Φ (? & ? & ->)) "HΦ".
+    wp_apply (wp_list_cons with "[//]").
+    iIntros (v' Hv').
+    iApply "HΦ".
+    iExists (_ :: _); eauto.
+  Qed.
+
+  Lemma wp_set_mem `{!Inj (=) (=) toval} ip x X v :
+    {{{ ⌜is_set X v⌝ }}}
+      set_mem (Val (toval x)) (Val v) @[ip]
+   {{{ (b : bool), RET #b; ⌜if b then x ∈ X else x ∉ X⌝ }}}.
+  Proof.
+    iIntros (Φ (l & ? & ->)) "HΦ".
+    iApply (wp_list_mem _ l with "[//]"); [done|].
+    iIntros ([] Hb); iApply "HΦ"; iPureIntro.
+    { set_solver. }
+    destruct Hb; set_solver.
+  Qed.
+
+End set_specs.
